Bisimilarity.v

theories/Bisimilarity.v
@@ -7,29 +7,32 @@ Section Definitions.
     {N : Set}
     (LTS2 : N -> A -> N -> Prop).
 
-  Record bisim_concl (Bisim : M -> N -> Prop) (t t' : N) (a : A) (s' : M) : Prop :=
-    { next_tr : LTS2 t a t';
-      next_bi : Bisim s' t'
-    }.
-
-  Record bisim_f (Bisim : M -> N -> Prop) (s : M) (t : N) : Prop :=
-    { bisim_l :
-        forall s' a,
-          LTS1 s a s' ->
-          exists t',
-            bisim_concl Bisim t t' a s';
-      bisim_r :
-        forall t' a,
-          LTS2 t a t' ->
-          exists s',
-            LTS1 s a s' /\ Bisim s' t';
-    }.
+  Definition simF (Sim : M -> N -> Prop) (s : M) (t : N) : Prop :=
+    forall s' a,
+      LTS1 s a s' ->
+      exists t',
+        LTS2 t a t' /\ Sim s' t'.
 
   Set Primitive Projections.
-  CoInductive bisim (s : M) (t : N) : Prop :=
-    In_bisim { out_bisim :  bisim_f bisim s t }.
+  CoInductive sim (s : M) (t : N) : Prop :=
+    In_sim { out_sim :  simF sim s t }.
   Unset Primitive Projections.
+
 End Definitions.
+
+Lemma sim_refl (M A : Set) (LTS : M -> A -> M -> Prop) (m : M)
+  : sim LTS LTS m m.
+Proof.
+  revert m.
+  cofix CH.
+  intros m.
+  constructor.
+  intros m' a tr.
+  exists m'.
+  split.
+  - exact tr.
+  - apply CH. Guarded.
+Qed.
 
 Section StreamExample.
    (* WARNING! We cannot do this with our approach because not an FSM *)
@@ -60,23 +63,163 @@ Definition zplus1 : stream nat := fmap S zeros.
 Inductive StreamLTS A : stream A -> A -> stream A -> Prop :=
 | stream_step : forall s x s', out_stream s = consF x s' -> StreamLTS A s x s'.
 
-(* Goal bisim (StreamLTS nat) (StreamLTS nat) zeros ones.
+Example stream_sim : sim (StreamLTS nat) (StreamLTS nat) zplus1 ones.
   cofix CH.
   constructor.
-  constructor.
-  - intros s' a H. inversion_clear H; subst.
-    inversion H0; subst.
-    exists ones, 1.
-    split.
-    apply stream_step; reflexivity.
-    apply CH.
-    Guarded.
-  - intros s' a H. inversion_clear H; subst.
-    inversion H0; subst.
-    exists zeros, 0.
-    split.
-    apply stream_step; reflexivity.
-    apply CH.
-    Guarded.
-  Qed. *)
+  intros s' a H. inversion_clear H; subst.
+  inversion H0; subst.
+  exists ones.
+  split.
+  apply stream_step; reflexivity.
+  apply CH. Guarded.
+Qed.
+
 End StreamExample.
+
+Module BisimTest1.
+  Inductive action : Set := | TheAction1 | TheAction2.
+  Inductive term : Set :=
+  | trec : term
+  | tend : term
+  | tfix : term -> term
+  | tact : action -> term -> term
+  | tpar : action -> action -> term -> term
+  .
+
+  Fixpoint subst (t1 : term) (t2 : term) :=
+    match t2 with
+    | trec => t1
+    | tend => tend
+    | tfix t => tfix t
+    | tact a t => tact a (subst t1 t)
+    | tpar a b t => tpar a b (subst t1 t)
+    end.
+
+  Inductive termLTS : term -> action -> term -> Prop :=
+  | do_act : forall a t, termLTS (tact a t) a t
+
+  | do_par1 : forall a b t, termLTS (tpar a b t) a (tact b t)
+
+  | do_par2 : forall a b t, termLTS (tpar a b t) b (tact a t)
+
+  | do_fix : forall a t t',
+      termLTS (subst (tfix t) t) a t' ->
+      termLTS (tfix t) a t'.
+
+  Ltac example_tactic CH :=
+   let r := fresh "r" in
+   let a := fresh "a" in
+   let tr := fresh "tr" in
+   constructor; intros r a tr;
+
+   (*  *)
+   repeat
+     match goal with
+     | [ H : termLTS ?l ?a ?r |- _ ] =>
+         inversion_clear H; simpl in *
+     end;
+   (*  *)
+
+   eexists;
+   split; [ repeat constructor | idtac ];
+   try apply sim_refl; try apply CH.
+
+  Ltac example_bisim :=
+    let CH := fresh "CH" in
+    cofix CH; repeat (example_tactic CH).
+
+  Goal sim termLTS termLTS
+    (tfix (tact TheAction1 trec))
+    (tact TheAction1 (tfix (tact TheAction1 trec))).
+  Proof.
+    example_bisim.
+  Qed.
+
+  Goal sim termLTS termLTS
+    (tact TheAction1 (tfix (tact TheAction1 trec)))
+    (tfix (tact TheAction1 trec)).
+  Proof.
+    example_bisim.
+  Qed.
+
+  Goal sim termLTS termLTS
+    (tfix (tact TheAction1 (tact TheAction2 trec)))
+    (tact TheAction1 (tfix (tact TheAction2 (tact TheAction1 trec)))).
+  Proof.
+    example_bisim.
+  Qed.
+
+  Goal sim
+    termLTS termLTS
+      (tfix (tpar TheAction1 TheAction2 trec))
+      (tfix (tpar TheAction1 TheAction2 trec)).
+    cofix CH.
+
+   let r := fresh "r" in
+   let a := fresh "a" in
+   let tr := fresh "tr" in
+   constructor; intros r a tr.
+   repeat
+     match goal with
+     | [ H : termLTS ?l ?a ?r |- _ ] =>
+         inversion_clear H; simpl in *
+     end.
+   eexists; split; [ repeat constructor | idtac ].
+   apply sim_refl.
+   simpl.
+
+   eexists.
+   split.
+   repeat constructor.
+   apply sim_refl.
+   Qed.
+
+  Section NonDetExamples.
+    Inductive Action := A | B.
+
+    Inductive TM1 := S | S1 | S2.
+    Inductive TM2 := T | T1.
+
+    Inductive LTS1 : TM1 -> Action -> TM1 -> Prop :=
+    | SS1A : LTS1 S A S1
+    | SS2A : LTS1 S A S2
+    | S1S2B : LTS1 S1 B S2
+    | S2S2B : LTS1 S2 B S2.
+
+    Inductive LTS2 : TM2 -> Action -> TM2 -> Prop :=
+    | TT1A : LTS2 T A T1
+    | T1T1A : LTS2 T1 A T1
+    | T1T1B : LTS2 T1 B T1.
+
+    Goal sim LTS2 LTS1 T S.
+      cofix CH.
+      constructor.
+      intros r a tr.
+      inversion_clear tr.
+      eexists.
+      split.
+      constructor.
+
+      cofix CH1.
+      constructor.
+      clear r a.
+      intros r a tr.
+      inversion_clear tr.
+      eexists.
+      Abort.
+    (*   split. *)
+    (*   constructor. *)
+
+    (*   cofix CH2. *)
+    (*   constructor. *)
+    (*   clear r a. *)
+    (*   intros r a tr. *)
+    (*   inversion_clear tr. *)
+    (*   eexists. *)
+    (*   split. *)
+    (*   constructor. *)
+    (*   apply CH2. *)
+    (* Qed. *)
+
+  End NonDetExamples.
+End BisimTest1.
